Switched from "half byte" to full byte, at the cost of a (very small) axiom

glue.ml
@@ -12,46 +12,284 @@
  * MERCHANTABILITY or FITNESS FOR A PARTICULAR PURPOSE.  See the GNU
  * General Public License for more details. *)
 
-
+open Byte
 open BinaryDefs
 open LazyList
 
 
-(* build a half byte from an int. This int *has* to be between 0 and
-   15 included. Fails loudly if it is not the case*)
+(* build a byte from an int. This int *has* to be between 0 and
+   255 included. Fails loudly if it is not the case*)
 
-let half_byte_of_int = function
-  | 0 -> HB0
-  | 1 -> HB1
-  | 2 -> HB2
-  | 3 -> HB3
-  | 4 -> HB4
-  | 5 -> HB5
-  | 6 -> HB6
-  | 7 -> HB7
-  | 8 -> HB8
-  | 9 -> HB9
-  | 10 -> HBA
-  | 11 -> HBB
-  | 12 -> HBC
-  | 13 -> HBD
-  | 14 -> HBE
-  | 15 -> HBF
+let byte_of_int = function
+  | 0 -> B00
+  | 1 -> B01
+  | 2 -> B02
+  | 3 -> B03
+  | 4 -> B04
+  | 5 -> B05
+  | 6 -> B06
+  | 7 -> B07
+  | 8 -> B08
+  | 9 -> B09
+  | 10 -> B0A
+  | 11 -> B0B
+  | 12 -> B0C
+  | 13 -> B0D
+  | 14 -> B0E
+  | 15 -> B0F
+  | 16 -> B10
+  | 17 -> B11
+  | 18 -> B12
+  | 19 -> B13
+  | 20 -> B14
+  | 21 -> B15
+  | 22 -> B16
+  | 23 -> B17
+  | 24 -> B18
+  | 25 -> B19
+  | 26 -> B1A
+  | 27 -> B1B
+  | 28 -> B1C
+  | 29 -> B1D
+  | 30 -> B1E
+  | 31 -> B1F
+  | 32 -> B20
+  | 33 -> B21
+  | 34 -> B22
+  | 35 -> B23
+  | 36 -> B24
+  | 37 -> B25
+  | 38 -> B26
+  | 39 -> B27
+  | 40 -> B28
+  | 41 -> B29
+  | 42 -> B2A
+  | 43 -> B2B
+  | 44 -> B2C
+  | 45 -> B2D
+  | 46 -> B2E
+  | 47 -> B2F
+  | 48 -> B30
+  | 49 -> B31
+  | 50 -> B32
+  | 51 -> B33
+  | 52 -> B34
+  | 53 -> B35
+  | 54 -> B36
+  | 55 -> B37
+  | 56 -> B38
+  | 57 -> B39
+  | 58 -> B3A
+  | 59 -> B3B
+  | 60 -> B3C
+  | 61 -> B3D
+  | 62 -> B3E
+  | 63 -> B3F
+  | 64 -> B40
+  | 65 -> B41
+  | 66 -> B42
+  | 67 -> B43
+  | 68 -> B44
+  | 69 -> B45
+  | 70 -> B46
+  | 71 -> B47
+  | 72 -> B48
+  | 73 -> B49
+  | 74 -> B4A
+  | 75 -> B4B
+  | 76 -> B4C
+  | 77 -> B4D
+  | 78 -> B4E
+  | 79 -> B4F
+  | 80 -> B50
+  | 81 -> B51
+  | 82 -> B52
+  | 83 -> B53
+  | 84 -> B54
+  | 85 -> B55
+  | 86 -> B56
+  | 87 -> B57
+  | 88 -> B58
+  | 89 -> B59
+  | 90 -> B5A
+  | 91 -> B5B
+  | 92 -> B5C
+  | 93 -> B5D
+  | 94 -> B5E
+  | 95 -> B5F
+  | 96 -> B60
+  | 97 -> B61
+  | 98 -> B62
+  | 99 -> B63
+  | 100 -> B64
+  | 101 -> B65
+  | 102 -> B66
+  | 103 -> B67
+  | 104 -> B68
+  | 105 -> B69
+  | 106 -> B6A
+  | 107 -> B6B
+  | 108 -> B6C
+  | 109 -> B6D
+  | 110 -> B6E
+  | 111 -> B6F
+  | 112 -> B70
+  | 113 -> B71
+  | 114 -> B72
+  | 115 -> B73
+  | 116 -> B74
+  | 117 -> B75
+  | 118 -> B76
+  | 119 -> B77
+  | 120 -> B78
+  | 121 -> B79
+  | 122 -> B7A
+  | 123 -> B7B
+  | 124 -> B7C
+  | 125 -> B7D
+  | 126 -> B7E
+  | 127 -> B7F
+  | 128 -> B80
+  | 129 -> B81
+  | 130 -> B82
+  | 131 -> B83
+  | 132 -> B84
+  | 133 -> B85
+  | 134 -> B86
+  | 135 -> B87
+  | 136 -> B88
+  | 137 -> B89
+  | 138 -> B8A
+  | 139 -> B8B
+  | 140 -> B8C
+  | 141 -> B8D
+  | 142 -> B8E
+  | 143 -> B8F
+  | 144 -> B90
+  | 145 -> B91
+  | 146 -> B92
+  | 147 -> B93
+  | 148 -> B94
+  | 149 -> B95
+  | 150 -> B96
+  | 151 -> B97
+  | 152 -> B98
+  | 153 -> B99
+  | 154 -> B9A
+  | 155 -> B9B
+  | 156 -> B9C
+  | 157 -> B9D
+  | 158 -> B9E
+  | 159 -> B9F
+  | 160 -> BA0
+  | 161 -> BA1
+  | 162 -> BA2
+  | 163 -> BA3
+  | 164 -> BA4
+  | 165 -> BA5
+  | 166 -> BA6
+  | 167 -> BA7
+  | 168 -> BA8
+  | 169 -> BA9
+  | 170 -> BAA
+  | 171 -> BAB
+  | 172 -> BAC
+  | 173 -> BAD
+  | 174 -> BAE
+  | 175 -> BAF
+  | 176 -> BB0
+  | 177 -> BB1
+  | 178 -> BB2
+  | 179 -> BB3
+  | 180 -> BB4
+  | 181 -> BB5
+  | 182 -> BB6
+  | 183 -> BB7
+  | 184 -> BB8
+  | 185 -> BB9
+  | 186 -> BBA
+  | 187 -> BBB
+  | 188 -> BBC
+  | 189 -> BBD
+  | 190 -> BBE
+  | 191 -> BBF
+  | 192 -> BC0
+  | 193 -> BC1
+  | 194 -> BC2
+  | 195 -> BC3
+  | 196 -> BC4
+  | 197 -> BC5
+  | 198 -> BC6
+  | 199 -> BC7
+  | 200 -> BC8
+  | 201 -> BC9
+  | 202 -> BCA
+  | 203 -> BCB
+  | 204 -> BCC
+  | 205 -> BCD
+  | 206 -> BCE
+  | 207 -> BCF
+  | 208 -> BD0
+  | 209 -> BD1
+  | 210 -> BD2
+  | 211 -> BD3
+  | 212 -> BD4
+  | 213 -> BD5
+  | 214 -> BD6
+  | 215 -> BD7
+  | 216 -> BD8
+  | 217 -> BD9
+  | 218 -> BDA
+  | 219 -> BDB
+  | 220 -> BDC
+  | 221 -> BDD
+  | 222 -> BDE
+  | 223 -> BDF
+  | 224 -> BE0
+  | 225 -> BE1
+  | 226 -> BE2
+  | 227 -> BE3
+  | 228 -> BE4
+  | 229 -> BE5
+  | 230 -> BE6
+  | 231 -> BE7
+  | 232 -> BE8
+  | 233 -> BE9
+  | 234 -> BEA
+  | 235 -> BEB
+  | 236 -> BEC
+  | 237 -> BED
+  | 238 -> BEE
+  | 239 -> BEF
+  | 240 -> BF0
+  | 241 -> BF1
+  | 242 -> BF2
+  | 243 -> BF3
+  | 244 -> BF4
+  | 245 -> BF5
+  | 246 -> BF6
+  | 247 -> BF7
+  | 248 -> BF8
+  | 249 -> BF9
+  | 250 -> BFA
+  | 251 -> BFB
+  | 252 -> BFC
+  | 253 -> BFD
+  | 254 -> BFE
+  | 255 -> BFF
   | _ -> assert false
 
 
 (* build a byte (pair of two half byte) from a char *)
 
 let byte_of_char c : byte =
-  let i = int_of_char c in
-  let hb1 = half_byte_of_int (i land 0xF) in
-  let hb2 = half_byte_of_int (i lsr 4) in
-  (hb2, hb1)
+  byte_of_int (int_of_char c)
+
 
 (* some unit test *)
-let _ = assert (byte_of_char (char_of_int 0xF0) = (HBF, HB0))
-let _ = assert (byte_of_char (char_of_int 0x1F) = (HB1, HBF))
-let _ = assert (byte_of_char (char_of_int 0x27) = (HB2, HB7))
+let _ = assert (byte_of_char (char_of_int 0xF0) = BF0)
+let _ = assert (byte_of_char (char_of_int 0x1F) = B1F)
+let _ = assert (byte_of_char (char_of_int 0x27) = B27)
 
 
 (* build the lazy list of bytes from an input channel *)
