TCB/BinaryDefs.v
@@ -15,54 +15,11 @@
 Require Import List.
 Require Import Lib.
 Require Import Omega.
+Require Export Byte.
 Open Scope positive_scope.
 Open Scope N_scope.
 
 
-(* Definition of a half byte *)
-
-Inductive half_byte :=
-| HB0
-| HB1
-| HB2
-| HB3
-| HB4
-| HB5
-| HB6
-| HB7
-| HB8
-| HB9
-| HBA
-| HBB
-| HBC
-| HBD
-| HBE
-| HBF.
-
-Lemma half_byte_eq_dec: eq_dec half_byte.
-Proof.
-  unfold eq_dec. decide equality.
-Qed.
-
-Definition N_of_half_byte hb : N:=
-  match hb with
-    | HB0 => 0
-    | HB1 => 1
-    | HB2 => 2
-    | HB3 => 3
-    | HB4 => 4
-    | HB5 => 5
-    | HB6 => 6
-    | HB7 => 7
-    | HB8 => 8
-    | HB9 => 9
-    | HBA => 10
-    | HBB => 11
-    | HBC => 12
-    | HBD => 13
-    | HBE => 14
-    | HBF => 15
-  end.
 
 (* add [trans] 0 bits *)
 
@@ -102,32 +59,275 @@ Proof.
 Qed.
 
 
-Definition concat_half_byte n hb := (translate_N_by_four n) + (N_of_half_byte hb).
-
-
-
-
-
-(* Bytes *)
-
-Definition byte := (half_byte * half_byte)%type.
-
-Lemma byte_eq_dec: eq_dec byte.
-Proof.
-  unfold eq_dec; decide equality; apply half_byte_eq_dec.
-Qed.
-
 Definition N_of_byte (b: byte) : N:=
-  concat_half_byte (N_of_half_byte (fst b)) (snd b).
+  match b with
+    | B00 => 0
+    | B01 => 1
+    | B02 => 2
+    | B03 => 3
+    | B04 => 4
+    | B05 => 5
+    | B06 => 6
+    | B07 => 7
+    | B08 => 8
+    | B09 => 9
+    | B0A => 10
+    | B0B => 11
+    | B0C => 12
+    | B0D => 13
+    | B0E => 14
+    | B0F => 15
+    | B10 => 16
+    | B11 => 17
+    | B12 => 18
+    | B13 => 19
+    | B14 => 20
+    | B15 => 21
+    | B16 => 22
+    | B17 => 23
+    | B18 => 24
+    | B19 => 25
+    | B1A => 26
+    | B1B => 27
+    | B1C => 28
+    | B1D => 29
+    | B1E => 30
+    | B1F => 31
+    | B20 => 32
+    | B21 => 33
+    | B22 => 34
+    | B23 => 35
+    | B24 => 36
+    | B25 => 37
+    | B26 => 38
+    | B27 => 39
+    | B28 => 40
+    | B29 => 41
+    | B2A => 42
+    | B2B => 43
+    | B2C => 44
+    | B2D => 45
+    | B2E => 46
+    | B2F => 47
+    | B30 => 48
+    | B31 => 49
+    | B32 => 50
+    | B33 => 51
+    | B34 => 52
+    | B35 => 53
+    | B36 => 54
+    | B37 => 55
+    | B38 => 56
+    | B39 => 57
+    | B3A => 58
+    | B3B => 59
+    | B3C => 60
+    | B3D => 61
+    | B3E => 62
+    | B3F => 63
+    | B40 => 64
+    | B41 => 65
+    | B42 => 66
+    | B43 => 67
+    | B44 => 68
+    | B45 => 69
+    | B46 => 70
+    | B47 => 71
+    | B48 => 72
+    | B49 => 73
+    | B4A => 74
+    | B4B => 75
+    | B4C => 76
+    | B4D => 77
+    | B4E => 78
+    | B4F => 79
+    | B50 => 80
+    | B51 => 81
+    | B52 => 82
+    | B53 => 83
+    | B54 => 84
+    | B55 => 85
+    | B56 => 86
+    | B57 => 87
+    | B58 => 88
+    | B59 => 89
+    | B5A => 90
+    | B5B => 91
+    | B5C => 92
+    | B5D => 93
+    | B5E => 94
+    | B5F => 95
+    | B60 => 96
+    | B61 => 97
+    | B62 => 98
+    | B63 => 99
+    | B64 => 100
+    | B65 => 101
+    | B66 => 102
+    | B67 => 103
+    | B68 => 104
+    | B69 => 105
+    | B6A => 106
+    | B6B => 107
+    | B6C => 108
+    | B6D => 109
+    | B6E => 110
+    | B6F => 111
+    | B70 => 112
+    | B71 => 113
+    | B72 => 114
+    | B73 => 115
+    | B74 => 116
+    | B75 => 117
+    | B76 => 118
+    | B77 => 119
+    | B78 => 120
+    | B79 => 121
+    | B7A => 122
+    | B7B => 123
+    | B7C => 124
+    | B7D => 125
+    | B7E => 126
+    | B7F => 127
+    | B80 => 128
+    | B81 => 129
+    | B82 => 130
+    | B83 => 131
+    | B84 => 132
+    | B85 => 133
+    | B86 => 134
+    | B87 => 135
+    | B88 => 136
+    | B89 => 137
+    | B8A => 138
+    | B8B => 139
+    | B8C => 140
+    | B8D => 141
+    | B8E => 142
+    | B8F => 143
+    | B90 => 144
+    | B91 => 145
+    | B92 => 146
+    | B93 => 147
+    | B94 => 148
+    | B95 => 149
+    | B96 => 150
+    | B97 => 151
+    | B98 => 152
+    | B99 => 153
+    | B9A => 154
+    | B9B => 155
+    | B9C => 156
+    | B9D => 157
+    | B9E => 158
+    | B9F => 159
+    | BA0 => 160
+    | BA1 => 161
+    | BA2 => 162
+    | BA3 => 163
+    | BA4 => 164
+    | BA5 => 165
+    | BA6 => 166
+    | BA7 => 167
+    | BA8 => 168
+    | BA9 => 169
+    | BAA => 170
+    | BAB => 171
+    | BAC => 172
+    | BAD => 173
+    | BAE => 174
+    | BAF => 175
+    | BB0 => 176
+    | BB1 => 177
+    | BB2 => 178
+    | BB3 => 179
+    | BB4 => 180
+    | BB5 => 181
+    | BB6 => 182
+    | BB7 => 183
+    | BB8 => 184
+    | BB9 => 185
+    | BBA => 186
+    | BBB => 187
+    | BBC => 188
+    | BBD => 189
+    | BBE => 190
+    | BBF => 191
+    | BC0 => 192
+    | BC1 => 193
+    | BC2 => 194
+    | BC3 => 195
+    | BC4 => 196
+    | BC5 => 197
+    | BC6 => 198
+    | BC7 => 199
+    | BC8 => 200
+    | BC9 => 201
+    | BCA => 202
+    | BCB => 203
+    | BCC => 204
+    | BCD => 205
+    | BCE => 206
+    | BCF => 207
+    | BD0 => 208
+    | BD1 => 209
+    | BD2 => 210
+    | BD3 => 211
+    | BD4 => 212
+    | BD5 => 213
+    | BD6 => 214
+    | BD7 => 215
+    | BD8 => 216
+    | BD9 => 217
+    | BDA => 218
+    | BDB => 219
+    | BDC => 220
+    | BDD => 221
+    | BDE => 222
+    | BDF => 223
+    | BE0 => 224
+    | BE1 => 225
+    | BE2 => 226
+    | BE3 => 227
+    | BE4 => 228
+    | BE5 => 229
+    | BE6 => 230
+    | BE7 => 231
+    | BE8 => 232
+    | BE9 => 233
+    | BEA => 234
+    | BEB => 235
+    | BEC => 236
+    | BED => 237
+    | BEE => 238
+    | BEF => 239
+    | BF0 => 240
+    | BF1 => 241
+    | BF2 => 242
+    | BF3 => 243
+    | BF4 => 244
+    | BF5 => 245
+    | BF6 => 246
+    | BF7 => 247
+    | BF8 => 248
+    | BF9 => 249
+    | BFA => 250
+    | BFB => 251
+    | BFC => 252
+    | BFD => 253
+    | BFE => 254
+    | BFF => 255
+  end.
 
-Definition byte0 : byte := (HB0, HB0).
+
+Definition byte0 : byte := B00.
 
 
-Goal N_of_byte (HB0,HB0) = 0.
+Goal N_of_byte B00 = 0.
   reflexivity. Qed.
-Goal N_of_byte (HB0,HB5) = 5.
+Goal N_of_byte B05 = 5.
   reflexivity. Qed.
-Goal N_of_byte (HB2,HB4) = 36.
+Goal N_of_byte B24 = 36.
   reflexivity. Qed.
 
 
@@ -153,7 +353,7 @@ Definition N_of_word w :=
   end.
 
 (* 0xDEADBEEF *)
-Goal N_of_word (W (HBD,HBE) (HBA,HBD) (HBB, HBE) (HBE, HBF)) = 3735928559.
+Goal N_of_word (W BDE BAD BBE BEF) = 3735928559.
   reflexivity. Qed.
 
 
